rocq-bluerock-brick/theories/lang/cpp/logic/monad.v
@@ -1,0 +1,753 @@
+(*
+ * Copyright (c) 2020-2024 BlueRock Security, Inc.
+ * This software is distributed under the terms of the BedRock Open-Source License.
+ * See the LICENSE-BedRock file in the repository root for details.
+ *)
+(** Definitions for the semantics
+ *)
+Require Import bedrock.prelude.base.
+
+Require Import stdpp.coPset.
+Require Import iris.bi.monpred.
+Require Import bedrock.lang.proofmode.proofmode.
+Require Import iris.proofmode.classes.
+
+Require Import bedrock.lang.cpp.syntax.
+Require Import bedrock.lang.cpp.semantics.
+Require Import bedrock.lang.cpp.logic.pred.
+Require Import bedrock.lang.cpp.logic.heap_pred.
+Require Import bedrock.lang.cpp.logic.translation_unit.
+Require Import bedrock.lang.bi.errors.
+
+#[local] Set Primitive Projections.
+
+(* expression continuations
+ * - in full C++, this includes exceptions, but our current semantics
+ *   doesn't treat those.
+ *)
+Definition epred `{cpp_logic} := mpred.
+Notation epredO := mpredO (only parsing).
+Bind Scope bi_scope with epred.
+
+Declare Scope free_scope.
+Delimit Scope free_scope with free.
+Reserved Infix "|*|" (at level 30).
+Reserved Infix ">*>" (at level 30).
+
+Require bedrock.lang.bi.linearity.
+Module FreeTemps.
+
+  (* BEGIN FreeTemps.t *)
+  Inductive t : Set :=
+  | id (* = fun x => x *)
+  | delete (ty : decltype) (p : ptr) (* = delete_val ty p *)
+           (* ^^ this type has qualifiers but is otherwise a runtime type *)
+  | delete_va (va : list (type * ptr)) (p : ptr)
+  | seq (f g : t) (* = fun x => f $ g x *)
+  | par (f g : t) (* = fun x => Exists Qf Qg, f Qf ** g Qg ** (Qf -* Qg -* x) *)
+  .
+  (* END FreeTemps.t *)
+
+  Module Import notations.
+    Bind Scope free_scope with t.
+    Notation "1" := id : free_scope.
+    Infix ">*>" := seq : free_scope.
+    Infix "|*|" := par : free_scope.
+  End notations.
+  #[local] Open Scope free_scope.
+
+  Inductive t_equiv : Equiv t :=
+  | refl l : l ≡ l
+  | sym l r : l ≡ r -> r ≡ l
+  | trans a b c : a ≡ b -> b ≡ c -> a ≡ c
+
+  | delete_ref ty p : delete (Tref ty) p ≡ delete (Trv_ref ty) p
+
+  | seqA x y z : x >*> (y >*> z) ≡ (x >*> y) >*> z
+  | seq_id_unitL l : 1 >*> l ≡ l
+  | seq_id_unitR l : l >*> 1 ≡ l
+  | seq_proper_ : ∀ {a b}, a ≡ b -> ∀ {c d}, c ≡ d -> a >*> c ≡ b >*> d
+
+  | parC l r : l |*| r ≡ r |*| l
+  | parA x y z : x |*| (y |*| z) ≡ (x |*| y) |*| z
+  | par_id_unitL l : 1 |*| l ≡ l
+  | par_proper_ : ∀ {a b}, a ≡ b -> ∀ {c d}, c ≡ d -> a |*| c ≡ b |*| d
+  .
+  Notation t_eq := (≡@{t}) (only parsing).
+
+  #[global] Existing Instance t_equiv.
+  #[global] Instance t_equivalence : Equivalence t_eq :=
+    Build_Equivalence _ refl sym trans.
+
+  #[global] Instance seq_assoc : Assoc equiv seq := seqA.
+  #[global] Instance seq_left_id : LeftId equiv id seq := seq_id_unitL.
+  #[global] Instance seq_right_id : RightId equiv id seq := seq_id_unitR.
+  #[global] Instance seq_proper : Proper (t_eq ==> t_eq ==> t_eq) seq := @seq_proper_.
+
+  #[global] Instance par_comm : Comm equiv par := parC.
+  #[global] Instance par_left_id : LeftId equiv id par := par_id_unitL.
+  #[global] Instance par_right_id : RightId equiv id par.
+  Proof. intros x. by rewrite comm left_id. Qed.
+  #[global] Instance par_proper : Proper (t_eq ==> t_eq ==> t_eq) par := @par_proper_.
+
+  (**
+  [pars ls] is the [FreeTemp] representing the destruction of each
+  element in [ls] *in non-deterministic order*.
+  *)
+  Definition pars : list t -> t := foldr par 1.
+
+  (**
+  [seqs ls] is the [FreeTemp] representing the destruction of each
+  element in [ls] sequentially from left-to-right, i.e. the first
+  element in the list is run first.
+  *)
+  Definition seqs : list t -> t := foldr seq 1.
+
+  (**
+  [seqs_rev ls] is the [FreeTemp] representing the destruction of each
+  element in [ls] sequentially from right-to-left, i.e. the first
+  element in the list is destructed last.
+  *)
+  Definition seqs_rev : list t -> t := foldl (fun a b => seq b a) 1.
+End FreeTemps.
+Export FreeTemps.notations.
+Notation FreeTemps := FreeTemps.t.
+Notation FreeTemp := FreeTemps.t (only parsing).
+
+(* continuations
+ * C++ statements can terminate in 4 ways.
+ *
+ * note(gmm): technically, they can also raise exceptions; however,
+ * our current semantics doesn't capture this. if we want to support
+ * exceptions, we should be able to add another case,
+ * `k_throw : val -> mpred`.
+ *)
+Variant ReturnType : Set :=
+| Normal
+| Break
+| Continue
+| ReturnVal (_ : ptr)
+| ReturnVoid
+.
+#[global] Instance ReturnType_ihn : Inhabited ReturnType.
+Proof. repeat constructor. Qed.
+
+Canonical Structure rt_biIndex : biIndex :=
+  {| bi_index_type := ReturnType
+   ; bi_index_rel := eq
+   |}.
+Definition KpredI `{!cpp_logic thread_info Σ} : bi := monPredI rt_biIndex (@mpredI thread_info Σ).
+#[global] Notation Kpred := (bi_car KpredI).
+
+Definition KP `{cpp_logic} (P : ReturnType -> mpred) : Kpred := MonPred P _.
+#[global] Arguments KP {_ _ _} _%_I : assert.
+#[global] Hint Opaque KP : typeclass_instances.
+
+Section KP.
+  Context `{Σ : cpp_logic}.
+
+  Lemma KP_frame (Q1 Q2 : ReturnType -> mpred) (rt : ReturnType) :
+    Q1 rt -* Q2 rt
+    |-- KP Q1 rt -* KP Q2 rt.
+  Proof. done. Qed.
+End KP.
+
+Definition Kat_exit `{Σ : cpp_logic} (Q : mpred -> mpred) (k : Kpred) : Kpred :=
+  KP $ fun rt => Q (k rt).
+#[global] Hint Opaque Kat_exit : typeclass_instances.
+
+Section Kat_exit.
+  Context `{Σ : cpp_logic}.
+
+  Lemma Kat_exit_frame (Q Q' : mpred -> mpred) (k k' : Kpred) :
+    Forall R R' : mpred, (R -* R') -* Q R -* Q' R' |--
+    Forall rt : ReturnType, (k rt -* k' rt) -*
+    Kat_exit Q k rt -* Kat_exit Q' k' rt.
+  Proof.
+    iIntros "HQ %rt Hk". destruct rt; cbn.
+    all: by iApply "HQ".
+  Qed.
+End Kat_exit.
+
+(*
+NOTE KpredI does not embed into mpredI because it doesn't respect
+existentials.
+*)
+#[global] Instance mpred_Kpred_BiEmbed `{Σ : cpp_logic} : BiEmbed mpredI KpredI := _.
+
+Section with_cpp.
+  Context `{Σ : cpp_logic}.
+
+  Import linearity.
+  (* the monad for expression evaluation *)
+  Record M {t : Type} :=
+    { _val : (t -> FreeTemps.t -> mpred) -> mpred
+    ; _ok : forall K1 K2, (Forall x free, K1 x free -* K2 x free) |-- _val K1 -* _val K2 }.
+  #[global] Arguments M _ : clear implicits.
+  #[local] Coercion _val : M >-> Funclass.
+
+  (* The canonical notion of equivalence on [M _]
+
+     This definition doesn't work, but it isn't clear how to fix it.
+     The issues:
+     - if you use pointwise equivalence for the [FreeTemps.t], then you
+       lose the monad laws.
+       You can get the bind-ret and ret-bind laws if you reify the unit,
+       but you can not get bind-bind.
+       **Idea**: use smart constructors that can canonicalize the definitions.
+     - if you use the equivalence on [FreeTemps.t], then you can not prove
+       this relation transitive because it requires that all functions satisfy
+       the equivalence.
+   *)
+  #[global] Instance M_equiv [T] : Equiv (M T) :=
+    (pointwise_relation _ ((≡) ==> (⊣⊢)) ==> (⊣⊢))%signature.
+  #[global] Instance M_equiv_refl {T} : Reflexive (≡@{M T}).
+  Proof.
+    repeat red. intros.
+    split'.
+    { iApply _ok; iIntros (??). rewrite H; eauto. }
+    { iApply _ok; iIntros (??). rewrite H; eauto. }
+  Qed.
+  #[global] Instance M_equiv_sym {T} : Symmetric (≡@{M T}).
+  Proof.
+    do 4 red; simpl; intros. symmetry. apply H.
+    red. red. intros. symmetry. apply H0. symmetry; eauto.
+  Qed.
+  #[global] Instance M_equiv_trans {T} : Transitive (≡@{M T}).
+  Proof.
+    do 4 red; simpl; intros. etrans. eapply H.  eapply H1.
+    eapply H0. red. red.
+    (* NOT PROVABLE! *)
+  Qed.
+
+
+  (* The canonical notation of approximation/entailment
+     Effectively, [a ⊆ b] if all behaviors of [a] are included in [b].
+   *)
+  #[global] Instance M_subseteq {T} : SubsetEq (M T) :=
+    (pointwise_relation _ (pointwise_relation _ (⊢)) ==> (⊢))%signature.
+
+  #[program]
+  Definition Mproduce (P : mpred) : M unit :=
+    {| _val := fun K => P -* K () FreeTemps.id |}.
+  Next Obligation.
+    intros; simpl. iIntros "X Y P". iApply "X". iApply "Y". iApply "P".
+  Qed.
+  #[program]
+  Definition Mconsume (P : mpred) : M unit :=
+    {| _val := fun K => P ** K () FreeTemps.id |}.
+  Next Obligation.
+    intros; simpl. iIntros "X [$ K]". iApply "X". iApply "K".
+  Qed.
+
+  Definition Massume (P : Prop) : M unit := Mproduce [| P |].
+  Definition Mrequire (P : Prop) : M unit := Mconsume [| P |].
+
+  #[program]
+  Definition Mret {t : Type} (v : t) : M t :=
+    {| _val K := K v FreeTemps.id |}.
+  Next Obligation.
+    intros; simpl. iIntros "X"; iApply "X".
+  Qed.
+
+  #[program]
+  Definition Mmap {t u : Type} (f : t -> u) (m : M t) : M u :=
+    {| _val K := m.(_val) (fun t => K (f t)) |}.
+  Next Obligation.
+    intros; simpl.
+    iIntros "X"; iApply _ok.
+    iIntros (??); iApply "X".
+  Qed.
+
+  #[program] Definition Mbind {T U} (c : M T) (k : T -> M U) : M U :=
+    {| _val K := c (fun v f => k v (fun v' f' => K v' (f' >*> f)%free)) |}.
+  Next Obligation.
+    simpl; intros. iIntros "K"; iApply _ok.
+    iIntros (??). iApply _ok. iIntros (??); iApply "K".
+  Qed.
+  Notation "'letWP*' v := e 'in' k" := (Mbind e (fun v => k)) (at level 0, v binder, k at level 200).
+
+  Lemma mret_mbind {T U} v (k : T -> M U) : Mbind (Mret v) k ≡ k v.
+  Proof.
+    red. rewrite /M_equiv/Mbind/Mret/=. red. simpl; intros.
+    split'.
+    { iApply _ok; iIntros (??).
+      rewrite H; eauto. apply FreeTemps.seq_id_unitR. }
+    { iApply _ok; iIntros (??).
+      rewrite H; eauto. apply FreeTemps.seq_id_unitR. }
+  Qed.
+
+  Lemma mbind_mret {T} (m : M T) : Mbind m Mret ≡ m.
+  Proof.
+    red; rewrite /M_equiv/Mbind/Mret; red; simpl; intros.
+    split'.
+    { iApply _ok; iIntros (??).
+      rewrite H. eauto. apply FreeTemps.seq_id_unitL. }
+    { iApply _ok; iIntros (??).
+      rewrite H. eauto. apply FreeTemps.seq_id_unitL. }
+  Qed.
+
+  Lemma mbind_mbind {T U V} (m : M T) (k1 : T -> M U) (k2 : U -> M V) :
+    Mbind m (fun x => Mbind (k1 x) k2) ≡ Mbind (Mbind m k1) k2.
+  Proof.
+    red; rewrite /M_equiv/Mbind; red; simpl; intros.
+    split';
+      iApply _ok; iIntros (??); iApply _ok; iIntros (??); iApply _ok; iIntros (??);
+      rewrite H; eauto.
+    all: by rewrite FreeTemps.seq_assoc.
+  Qed.
+
+  #[program]
+  Definition Mnd (t : Type) : M t :=
+    {| _val K := ∀ x : t, K x FreeTemps.id |}%I.
+  Next Obligation.
+    simpl; intros.
+    iIntros "K X" (?); iApply "K"; eauto.
+  Qed.
+  #[program]
+  Definition Mangelic (t : Type) : M t :=
+    {| _val K := ∃ x : t, K x FreeTemps.id |}%I.
+  Next Obligation.
+    simpl; intros.
+    iIntros "K X"; iDestruct "X" as (?) "X"; iExists _; iApply "K"; eauto.
+  Qed.
+
+  #[program]
+  Definition Mub {t : Type} : M t :=
+    {| _val _ := False%I |}.
+  Next Obligation. simpl; intros. iIntros "? []". Qed.
+  #[program]
+  Definition Many {t : Type} : M t :=
+    {| _val _ := True%I |}.
+  Next Obligation. simpl; intros; iIntros "? ?". iApply bi.pure_intro; [ trivial | ]. iStopProof. reflexivity. Qed.
+
+  #[program]
+  Definition Merror {t : Type} {ERR : Type} (err : ERR) : M t :=
+    {| _val _ := ERROR err |}.
+  Next Obligation. simpl; intros. rewrite ERROR_False. iIntros "? []". Qed.
+
+  #[program]
+  Definition Mpush_free (f : FreeTemps.t) : M () :=
+    {| _val K := K () f |}.
+  Next Obligation. simpl; intros. iIntros "K"; iApply "K". Qed.
+
+  #[program]
+  Definition Matomically {t} (m : M t) : M t :=
+    {| _val K := |={top,∅}=> m.(_val) (fun r free => |={∅,top}=> K r free) |}%I.
+  Next Obligation.
+    simpl; intros. iIntros "K >X !>"; iRevert "X".
+    iApply _ok. iIntros (??) ">X !>"; iRevert "X"; iApply "K".
+  Qed.
+
+  #[program]
+  Definition Mnon_atomically {t} (m : M t) : M t :=
+    {| _val K := |={top}=> m.(_val) (fun r free => |={top}=> K r free) |}%I.
+  Next Obligation.
+    simpl; intros. iIntros "K >X !>"; iRevert "X".
+    iApply _ok. iIntros (??) ">X !>"; iRevert "X"; iApply "K".
+  Qed.
+
+  #[program]
+  Definition Mfupd (E1 E2 : coPset): M unit :=
+    {| _val K := |={E1,E2}=> K () FreeTemps.id |}%I.
+  Next Obligation.
+    simpl; intros. iIntros "K >X !>"; iRevert "X"; iApply "K".
+  Qed.
+
+  #[program]
+  Definition Mstable : M unit :=
+    {| _val K := |={top}=> K () FreeTemps.id |}%I.
+  Next Obligation.
+    simpl; intros. iIntros "K >X !>"; iRevert "X"; iApply "K".
+  Qed.
+
+  #[program]
+  Definition Mboth {t} (a b : M t) : M t :=
+    {| _val K := a K //\\ b K |}.
+  Next Obligation.
+    simpl; intros. iIntros "K X".
+    iSplit; [ iDestruct "X" as "[X _]" | iDestruct "X" as "[_ X]" ]; iRevert "X"; iApply _ok; iIntros (??); iApply "K".
+  Qed.
+
+  (*
+  Definition Mread {t} (R : t -> mpred) : M t :=
+    MonPred (I:=M_index t) (fun K => Exists v, R v ** (R v -* K v FreeTemps.id)) _.
+  Definition Mread_with {TT : tele} (R : TT -t> mpred) : M TT :=
+    MonPred (I:=M_index TT) (fun K => ∃.. v, tele_app R v ** (tele_app R v -* K v FreeTemps.id))%I _.
+   *)
+
+  Definition Mframe {T} (a b : M T) : mpred :=
+    Forall Q Q', (Forall x y, Q x y -* Q' x y) -* a Q -* b Q'.
+
+  Definition WP {T} (m : M T) (Q : T -> FreeTemps.t -> mpred) : mpred :=
+    m Q.
+
+  Definition Mimpl {T} (a b : M T) : mpred :=
+    ∀ Q, a Q -* b Q.
+
+  Lemma WP_impl {T} (a b : M T) Q : Mimpl a b |-- WP a Q -* WP b Q.
+  Proof. rewrite /Mimpl. iIntros "X". iApply "X". Qed.
+
+  Lemma Mmap_frame_strong {T U} c (f : T -> U) :
+    Mframe c c
+    |-- Forall Q Q', (Forall x y, Q (f x) y -* Q' (f x) y) -* Mmap f c Q -* Mmap f c Q'.
+  Proof.
+    rewrite /Mframe/Mmap; iIntros "A" (??) "B".
+    iApply "A". iIntros (??); iApply "B".
+  Qed.
+
+  Lemma Mmap_frame {T U} c1 c2 (f : T -> U) :
+    Mframe c1 c2 |-- Mframe (Mmap f c1) (Mmap f c2).
+  Proof.
+    rewrite /Mframe/Mmap; iIntros "A" (??) "B".
+    iApply "A". iIntros (??); iApply "B".
+  Qed.
+
+
+  Lemma Mframe_refl {T} (m : M T) : |-- Mframe m m.
+  Proof.
+    rewrite /Mframe. iIntros (??) "X".
+    iApply _ok. eauto.
+  Qed.
+
+  Lemma Mbind_frame {T U} c1 c2 (k1 k2 : T -> M U) :
+    Mframe c1 c2 |-- (Forall x, Mframe (k1 x) (k2 x)) -* Mframe (Mbind c1 k1) (Mbind c2 k2).
+  Proof.
+    rewrite /Mframe/Mbind; iIntros "A B" (??) "C".
+    iApply "A". iIntros (??). iApply "B".
+    iIntros (??); iApply "C".
+  Qed.
+
+  (** *** Indeterminately sequenced computations
+      Note that [FreeTemps.t] is sequenced in reverse order of construction
+      to encode the stack discipline guaranteed by C++.
+      (CITATION NEEDED)
+   *)
+  #[program]
+  Definition nd_seq {T U} (wp1 : M T) (wp2 : M U) : M (T * U) :=
+    Mboth (letWP* v1 := wp1 in
+           letWP* v2 := wp2 in
+           Mret (v1,v2))
+          (letWP* v2 := wp2 in
+           letWP* v1 := wp1 in
+           Mret (v1,v2)).
+
+  Lemma nd_seq_frame {T U} wp1 wp2 :
+    Mframe wp1 wp1 |-- Mframe wp2 wp2 -* Mframe (@nd_seq T U wp1 wp2) (nd_seq wp1 wp2).
+  Proof.
+    iIntros "A B" (??) "C D".
+    iSplit; [ iDestruct "D" as "[D _]" | iDestruct "D" as "[_ D]" ]; iRevert "D".
+    { iApply "A". iIntros (??). iApply "B"; iIntros (??). iApply "C". }
+    { iApply "B". iIntros (??). iApply "A"; iIntros (??). iApply "C". }
+  Qed.
+
+  (* Lifting non-deterministic sequencing to lists.
+
+     NOTE: this is like the semantics of argument evaluation in C++.
+   *)
+  (*
+  Fixpoint nd_seqs' {T} (f : nat) (qs : list (M T)) {struct f} : M (list T) :=
+    match qs with
+    | nil => Mret nil
+    | _ :: _ =>
+      match f with
+      | 0 => Mub
+      | S f => fun Q =>
+        Forall pre post q, [| qs = pre ++ q :: post |] -*
+               let lpre := length pre in
+               Mbind q (fun t => Mmap (fun ts => firstn lpre ts ++ t :: skipn lpre ts) (nd_seqs' f (pre ++ post))) Q
+      end
+    end.
+   *)
+
+  Definition nd_seqs {T} (qs : list (M T)) : M (list T). (* := @nd_seqs' T (length qs) qs. *) Admitted.
+
+  (*
+  Lemma nd_seqs'_frame_strong {T} n : forall (ls : list (M T)) Q Q',
+      n = length ls ->
+      Forall x y, [| length x = length ls |] -* Q x y -* Q' x y
+      |-- ([∗list] m ∈ ls, Mframe m m) -*
+          nd_seqs' n ls Q -* nd_seqs' n ls Q'.
+  Proof.
+    induction n; simpl; intros.
+    { case_match; eauto.
+      subst. simpl.
+      iIntros "X _". iApply "X". eauto. }
+    { destruct ls. exfalso; simpl in *; congruence.
+      inversion H.
+      iIntros "X LS Y" (???) "%P".
+      iSpecialize ("Y" $! pre).
+      iSpecialize ("Y" $! post).
+      iSpecialize ("Y" $! q).
+      iDestruct ("Y" with "[]") as "Y"; first eauto.
+      rewrite P.
+      iDestruct "LS" as "(a&b&c)".
+      iRevert "Y". rewrite /Mbind.
+      iApply "b".
+      iIntros (??).
+      rewrite /Mmap.
+      subst.
+      assert (length ls = length (pre ++ post)).
+      { have: (length (m :: ls) = length (pre ++ q :: post)) by rewrite P.
+        rewrite !length_app /=. lia. }
+      iDestruct (IHn with "[X]") as "X". eassumption.
+      2:{
+      iDestruct ("X" with "[a c]") as "X".
+      iSplitL "a"; eauto.
+      iApply "X". }
+      simpl. iIntros (??) "%". iApply "X".
+      revert H0 H1. rewrite !length_app/=.
+      intros. iPureIntro.
+      rewrite firstn_length_le; last lia.
+      rewrite length_skipn. lia. }
+  Qed.
+
+  Lemma nd_seqs'_frame {T} n : forall (ls : list (M T)),
+      n = length ls ->
+      ([∗list] m ∈ ls, Mframe m m)
+      |-- Mframe (nd_seqs' n ls) (nd_seqs' n ls).
+  Proof.
+    induction n; simpl; intros.
+    { case_match.
+      { subst. simpl.
+        iIntros "_" (??) "X". iApply "X". }
+      { iIntros "?" (??) "? []". } }
+    { destruct ls. exfalso; simpl in *; congruence.
+      inversion H.
+      iIntros "LS" (??) "X Y"; iIntros (???) "%P".
+      iSpecialize ("Y" $! pre).
+      iSpecialize ("Y" $! post).
+      iSpecialize ("Y" $! q).
+      iDestruct ("Y" with "[]") as "Y"; first eauto.
+      rewrite P.
+      iDestruct "LS" as "(a&b&c)".
+      iRevert "Y".
+      iApply (Mbind_frame with "b [a c]"); eauto.
+      iIntros (?).
+      iApply Mmap_frame.
+      rewrite -H1.
+      iApply IHn.
+      { have: (length (m :: ls) = length (pre ++ q :: post)) by rewrite P.
+        rewrite !length_app /=. lia. }
+      iSplitL "a"; eauto. }
+  Qed.
+  Lemma nd_seqs_frame : forall {T} (ms : list (_ T)),
+      ([∗list] m ∈ ms, Mframe m m) |-- Mframe (nd_seqs ms) (nd_seqs ms).
+  Proof. intros. by iApply nd_seqs'_frame. Qed.
+
+  (* sanity check on [nd_seq] and [nd_seqs] *)
+  Example nd_seq_example : forall {T} (a b : M T),
+      Proper (Mrel _) a -> Proper (Mrel _) b ->
+      Mequiv _ (nd_seqs [a;b]) (Mmap (fun '(a,b) => [a;b]) $ nd_seq a b).
+  Proof.
+    rewrite /nd_seqs/=; intros.
+    rewrite /Mmap/nd_seq.
+    repeat intro.
+    iSplit.
+    { iIntros "X".
+      iSplit.
+      { iSpecialize ("X" $! nil [b] a eq_refl).
+        iRevert "X".
+        iApply H. repeat intro; simpl.
+        iIntros "X".
+        iSpecialize ("X" $! nil nil b eq_refl).
+        iRevert "X".
+        iApply H0. repeat intro; simpl.
+        rewrite /Mret.
+        rewrite (H1 _ _ _) => //. by rewrite FreeTemps.seq_id_unitL. }
+      { iSpecialize ("X" $! [a] nil b eq_refl).
+        iRevert "X". iApply H0. repeat intro; simpl.
+        iIntros "X".
+        iSpecialize ("X" $! nil nil a eq_refl).
+        iRevert "X".
+        iApply H. repeat intro; simpl.
+        rewrite /Mret.
+        rewrite H1 => //. by rewrite FreeTemps.seq_id_unitL. } }
+    { iIntros "X" (pre post m Horder).
+      destruct pre.
+      { inversion Horder; subst.
+        iDestruct "X" as "[X _]".
+        rewrite /Mbind. iApply H; last iAssumption.
+        iIntros (??) => /=.
+        iIntros "X" (pre' post' m' Horder').
+        assert (pre' = [] /\ m' = b /\ post' = []) as [?[??]]; last subst.
+        { clear - Horder'.
+          destruct pre'.
+          - inversion Horder'; subst; auto.
+          - destruct pre'; inversion Horder'. }
+        iApply H0; last iAssumption.
+        iIntros (??) => /=; rewrite /Mret/=.
+        rewrite H1 => //. by rewrite FreeTemps.seq_id_unitL. }
+      { assert (a = m0 /\ b = m /\ pre = [] /\ post = []) as [?[?[??]]]; last subst.
+        { clear -Horder.
+          inversion Horder; subst.
+          destruct pre; inversion H1; subst; eauto.
+          destruct pre; inversion H2. }
+        iDestruct "X" as "[_ X]".
+        rewrite /Mbind. iApply H0; last iAssumption.
+        iIntros (??) "H" => /=. iIntros (pre' post' m' Horder')=> /=.
+        assert (m0 = m' /\ pre' = [] /\ post' = []) as [?[??]]; last subst.
+        { destruct pre'; inversion Horder'; subst; eauto.
+          destruct pre'; inversion H4. }
+        iApply H; last iAssumption.
+        iIntros (??). rewrite /=/Mret/=.
+        rewrite H1 => //.
+        by rewrite FreeTemps.seq_id_unitL. } }
+  Qed.
+  *)
+
+  (** *** sequencing of monadic compuations *)
+  Definition Mseq {T U} (wp1 : M T) (wp2 : M U) : M (T * U) :=
+    Mbind wp1 (fun v => Mmap (fun x => (v, x)) wp2).
+
+  Lemma Mseq_frame {T U} wp1 wp2 :
+    Mframe wp1 wp1 |-- Mframe wp2 wp2 -* Mframe (@Mseq T U wp1 wp2) (Mseq wp1 wp2).
+  Proof.
+    iIntros "A B" (??) "C".
+    rewrite /Mseq.
+    iApply (Mbind_frame with "A [B]"); last iAssumption.
+    iIntros (???) "X". iApply (Mmap_frame with "B"). done.
+  Qed.
+
+  (** [seqs es] is sequential evaluation of [es] *)
+  Fixpoint seqs {T} (es : list (M T)) : M (list T) :=
+    match es with
+    | nil => Mret []
+    | e :: es => Mmap (fun '(a,b) => a:: b) (Mseq e (seqs es))
+    end.
+
+  Lemma seqs_frame_strong {T} : forall (ls : list (M T)) Q Q',
+      ([∗list] m ∈ ls, Mframe m m)%I
+      |-- (Forall x y, [| length x = length ls |] -* Q x y -* Q' x y) -*
+          (seqs ls Q) -* (seqs ls Q').
+  Proof.
+    induction ls; simpl; intros.
+    - iIntros "_ X"; iApply "X"; eauto.
+    - iIntros "[A AS] K".
+      rewrite /Mbind. iApply "A".
+      iIntros (??).
+      iApply (IHls with "AS").
+      iIntros (???).
+      iApply "K". simpl. eauto.
+  Qed.
+
+  (** *** interleaving of monadic values
+
+      We encode interleaving through concurrency which we represent through
+      separable resources.
+
+      NOTE: this is like the semantics of argument evaluation in C
+   *)
+  #[program]
+  Definition Mpar {T U} (wp1 : M T) (wp2 : M U) : M (T * U) :=
+    {| _val K := Exists Q1 Q2, wp1 Q1 ** wp2 Q2 ** (Forall v1 v2 f1 f2, Q1 v1 f1 -* Q2 v2 f2 -* K (v1,v2) (f1 |*| f2)%free) |}.
+  Next Obligation.
+    simpl; intros.
+    iIntros "K X". iDestruct "X" as (??) "[? [? Q]]".
+    iExists _, _; iFrame. iIntros (????) "Q1 Q2". iApply "K". iApply ("Q" with "Q1 Q2").
+  Qed.
+
+  Lemma Mpar_frame {T U} wp1 wp2 :
+    Mframe wp1 wp1 |-- Mframe wp2 wp2 -* Mframe (@Mpar T U wp1 wp2) (Mpar wp1 wp2).
+  Proof.
+    iIntros "A B" (??) "C D".
+    rewrite /Mpar/Mframe.
+    iDestruct "D" as (??) "(D1 & D2 & K)".
+    iExists _, _.
+    iSplitL "D1 A".
+    iApply "A". 2: eauto. iIntros (??) "X"; iApply "X".
+    iSplitL "D2 B".
+    iApply "B". 2: eauto. iIntros (??) "X"; iApply "X".
+    iIntros (????) "A B". iApply "C". iApply ("K" with "A B").
+  Qed.
+
+
+  (** lifting [Mpar] to homogeneous lists *)
+  Fixpoint Mpars {T} (f : list (M T)) : M (list T) :=
+    match f with
+    | nil => Mret nil
+    | f :: fs => Mmap (fun '(v, vs) => v :: vs) $ Mpar f (Mpars fs)
+    end.
+
+  Lemma Mpars_frame_strong {T} : forall (ls : list (M T)) Q Q',
+      |-- (Forall x y, [| length x = length ls |] -* Q x y -* Q' x y) -*
+          (Mpars ls Q) -* (Mpars ls Q').
+  Proof.
+    induction ls; simpl; intros.
+    - iIntros "X"; iApply "X"; eauto.
+    - iIntros "K".
+      rewrite /Mmap.
+      rewrite /Mpar.
+      iIntros "X".
+      iDestruct "X" as (??) "(L & R & KK)".
+      iExists _, _. iFrame "L".
+      iDestruct (IHls with "[] R") as "IH".
+      2: iFrame "IH".
+      { instantiate (1:=fun x y => [| length x = length ls |] ** Q2 x y).
+        iIntros (???) "$". eauto. }
+      iIntros (????) "? [% ?]".
+      iApply "K".
+      { simpl. eauto. }
+      iApply ("KK" with "[$] [$]").
+  Qed.
+
+  (** *** evaluation by a scheme *)
+
+  (** [eval eo e1 e2] evaluates [e1], [e2] according to the evaluation scheme [eo] *)
+  Definition eval2 (eo : evaluation_order.t) {T U} (e1 : M T) (e2 : M U) : M (T * U) :=
+    match eo with
+    | evaluation_order.nd => nd_seq e1 e2
+    | evaluation_order.l_nd => Mseq e1 e2
+    | evaluation_order.rl => Mmap (fun '(a,b) => (b,a)) $ Mseq e2 e1
+    end.
+
+  (** [evals eo es] evaluates [es] according to the evaluation scheme [eo] *)
+  Definition eval (eo : evaluation_order.t) {T} (es : list (M T)) : M (list T) :=
+    match eo with
+    | evaluation_order.nd => nd_seqs es
+    | evaluation_order.l_nd =>
+        match es with
+        | e :: es => Mbind e (fun v => Mmap (fun vs => v :: vs) (nd_seqs es))
+        | [] => Mret []
+        end
+    | evaluation_order.rl => Mmap (@rev _) (seqs (rev es))
+    end.
+
+  Lemma eval_frame_strong {T} oe : forall (ls : list (M T)) Q Q',
+      ([∗list] m ∈ ls, Mframe m m)%I
+      |-- (Forall x y, [| length x = length ls |] -* Q x y -* Q' x y) -*
+          eval oe ls Q -* eval oe ls Q'.
+  Proof. (*
+    destruct oe; intros.
+    - rewrite /=/nd_seqs. iIntros "A B".
+      iApply (nd_seqs'_frame_strong with "B A"). done.
+    - simpl.
+      destruct ls; simpl.
+      { iIntros "_ X"; iApply "X". done. }
+      { iIntros "[X Y] K".
+        iApply "X". iIntros (??).
+        iApply (nd_seqs'_frame_strong with "[K] Y"); eauto.
+        iIntros (???).
+        rewrite /Mret.
+        iApply "K". simpl; eauto. }
+    - simpl.
+      iIntros "X K".
+      rewrite /Mmap. iApply (seqs_frame_strong with "[X]").
+      { iStopProof. induction ls; simpl; eauto.
+        iIntros "[$ K]".
+        iDestruct (IHls with "K") as "$". eauto. }
+      { iIntros (???); iApply "K".
+        rewrite length_rev. eauto. rewrite -(length_rev ls). eauto. }
+  Qed. *) Admitted.
+
+  Fixpoint tuple (ts : list Type) : Type :=
+    match ts return Type with
+    | nil => unit
+    | t :: ts => t * tuple ts
+    end.
+
+  (* TODO: this is the heterogeneous extension of [eval] *)
+  Parameter heval : forall (eo : evaluation_order.t) {ts} (x : tuple (M <$> ts)), M (tuple ts).
+End with_cpp.
+
+Notation "'letWP*' v := e 'in' k" := (Mbind e (fun v => k)) (at level 0, v binder, k at level 200).
